@prefix rdf: <http://www.w3.org/1999/02/22-rdf-syntax-ns#> .
@prefix rdfs: <http://www.w3.org/2000/01/rdf-schema#> .
@prefix owl: <http://www.w3.org/2002/07/owl#> .
@prefix dcterms: <http://purl.org/dc/terms/> .
@prefix vann: <http://purl.org/vocab/vann/> .
@prefix xsd: <http://www.w3.org/2001/XMLSchema#> .
@prefix vcard: <https://www.w3.org/TR/vcard-rdf/> .

@prefix fitp: <https://jeffreywallphd.github.io/vocab/fitp.ttl#> .
@prefix athl: <https://jeffreywallphd.github.io/vocab/athl.ttl#> .

#TODO: create a separate FitnessGoal vocabulary to describe fitness goals

#TODO: change the name of this vocabulary to fitp for fitness program
fitp: a owl:Ontology ;
    owl:versionInfo "0.0.1" ;
    dcterms:creator "Jeffrey Wall" ;
    dcterms:date "2023-10-03" ;
    dcterms:title "Fitness Program Vocabulary" ;
    dcterms:description "A vocabulary for describing physical fitness programs"@en ;
    vann:preferredNamespacePrefix "fitp" ;
    vann:preferredNamespaceUri "https://jeffreywallphd.github.io/vocab/fitp.ttl#" .

# Classes
fitp:Athlete rdf:type rdfs:Class ;
    rdfs:label "Athlete" ;
    rdfs:comment "A person that performs physical activity" ;
    rdfs:subClassOf athl:Athlete .

fitp:Coach rdf:type rdfs:Class ;
    rdfs:label "Coach" ;
    rdfs:comment "A person who coaches an #Athlete" ;
    rdfs:subClassOf athl:Coach .

fitp:Program rdf:type rdf:Seq ;
    rdfs:label "Fitness Program" ;
    rdfs:comment "A generic fitness program or workout consisting of a sequence of exercises" .

fitp:Curcuit rdf:type rdf:Seq ;
    rdfs:label "Circuit Training" ;
    rdfs:comment "A fitness program that includes rotating through a variety of exercises in a particular sequence" ;
    rdfs:subClassOf fitp:Program .

fitp:Drill rdf:type rdf:Seq ;
    rdfs:label "Fitness Drill" ;
    rdfs:comment "A fitness program that includes repetitive, sequential activity to produce disciplined performance" ;
    rdfs:subClassOf fitp:Program .

fitp:Exercise rdf:type rdfs:Class ;
    rdfs:label "Exercise Activity" ;
    rdfs:comment "A physical activity, often a part of a fitness #Program, performed by an #Athlete" .

fitp:Set rdf:type rdfs:Class ;
    rdfs:label "Set" ;
    rdfs:comment "A set of a particular #Exercise" .

fitp:Rep rdf:type rdfs:Class ;
    rdfs:label "Rep" ;
    rdfs:comment "A rep of a particular #Set of an #Exercise" .

# Properties
fitp:assignedBy rdf:type rdf:Property ;
    rdfs:label "assigned by" ;
    rdfs:comment "An #Program assigned by a #Coach" ;
    rdfs:domain (fitp:Program) ;
    rdfs:range (fitp:Coach) .

fitp:assignedTo rdf:type rdf:Property ;
    rdfs:label "assigned to" ;
    rdfs:comment "An assignment of a #Program to an #Athlete" ;
    rdfs:domain (fitp:Program) ;
    rdfs:range (fitp:Athlete) .

fitp:name rdf:type rdfs:Property ;
    rdfs:label "name" ;
    rdfs:comment "A name given to a #Program or #Program subtype, #Excerise, and other named fitp classes" ;
    rdfs:domain (fitp:Program fitp:Exercise) ;
    rdfs:range (xsd:string) .

fitp:description rdf:type rdfs:Property ;
    rdfs:label "description" ;
    rdfs:comment "A description of a #Program or #Exercise" ;
    rdfs:domain (fitp:Program fitp:Exercise);
    rdfs:range (xsd:string) .

#This no longer seems necessary after changing Program to a Sequence of #Exercises
#fitp:consistsOf rdf:type rdf:Property ;
#    rdfs:label "consists of" ;
#    rdfs:comment "A property to designate that a #Program or #Program sub-class consists of #Excercise, an #Exercise of #Set, or a #Set of #Rep" ;
#    rdfs:domain (fitp:Program fitp:Exercise fitp:Set) ;
#    rdfs:range (fitp:Exercise fitp:Set fitp:Rep) .

# TODO: consider moving this attribute to a fitness record vocabulary to differentiate a routine from engagement in a routine
fitp:performedBy rdf:type rdf:Property ;
    rdfs:label "performed by" ;
    rdfs:comment "A property to designate that an #Athlete performed an #Exercise" ;
    rdfs:domain (fitp:Athlete) ;
    rdfs:range (fitp:Rep) .

fitp:repType rdf:type rdfs:Property ;
    rdfs:label "rep type" ;
    rdfs:comment "A type of #Rep, such as weight, distance, time, or simple quantity" ;
    rdfs:domain (fitp:Rep) ;
    rdfs:range (xsd:string) .

fitp:quantity rdf:type rdfs:Property ;
    rdfs:label "quantity" ;
    rdfs:comment "A quantity of #Set or #Rep" ;
    rdfs:domain (fitp:Set fitp:Rep) ;
    rdfs:range (xsd:integer) .

fitp:weight rdf:type rdfs:Property ;
    rdfs:label "weight" ;
    rdfs:comment "A weight value of a or #Rep" ;
    rdfs:domain (fitp:Rep) ;
    rdfs:range (xsd:float) .

fitp:weightMetric rdfs:subPropertyOf fitp:weight ;
    rdfs:label "weight metric" ;
    rdfs:comment "a weight metric, such as pounds or kilos" ;
    rdfs:range (xsd:string) .

fitp:distance rdf:type rdfs:Property ;
    rdfs:label "distance" ;
    rdfs:comment "A distance value of a #Rep" ;
    rdfs:domain (fitp:Rep) ;
    rdfs:range (xsd:float) .

fitp:distanceMetric rdfs:subPropertyOf fitp:distance ;
    rdfs:label "distance metric" ;
    rdfs:comment "a distance metric, such as feet, yards, miles, meters, kilometers" ;
    rdfs:range (xsd:string) .

fitp:time rdf:type rdfs:Property ;
    rdfs:label "time" ;
    rdfs:comment "A time value of a #Rep" ;
    rdfs:domain (fitp:Rep) ;
    rdfs:range (xsd:float) .

fitp:timeMetric rdfs:subPropertyOf fitp:time ;
    rdfs:label "time metric" ;
    rdfs:comment "a time metric, such as seconds, minutes, hours" ;
    rdfs:range (xsd:string) .